new/golang/theory/exception.v
@@ -1,5 +1,8 @@
 From New.golang.defn Require Export exception.
-From New.golang.theory Require Export pure_proofmode.
+From New.golang.theory Require Export pure_proofmode typing.
+From iris.proofmode Require Import coq_tactics.
+Import Ltac2.
+Set Default Proof Mode "Classic".
 
 Section wps.
 Context `{sem: ffi_semantics} `{!ffi_interp ffi} `{!heapGS Σ}.
@@ -9,14 +12,14 @@ Global Instance pure_execute_val (v1 : val) (v : val) :
 Proof.
   rewrite exception_seq_unseal execute_val_unseal.
   intros ?????. iIntros "Hwp".
-  wp_rec. wp_pures. iFrame.
+  wp_call. iFrame.
 Qed.
 
 Global Instance pure_do_execute_val (v : val) : PureWp True (do: v) (execute_val v).
 Proof.
   rewrite do_execute_unseal execute_val_unseal.
   intros ?????. iIntros "Hwp".
-  wp_rec. wp_pures. iFrame.
+  wp_call. iFrame.
 Qed.
 
 Global Instance pure_return_val (v1 : val) (v : val) :
@@ -24,21 +27,21 @@ Global Instance pure_return_val (v1 : val) (v : val) :
 Proof.
   rewrite exception_seq_unseal return_val_unseal.
   intros ?????. iIntros "Hwp".
-  wp_rec. wp_pures. iFrame.
+  wp_call. iFrame.
 Qed.
 
 Global Instance pure_do_return_val (v : val) : PureWp True (return: v) (return_val v).
 Proof.
   rewrite do_return_unseal return_val_unseal.
   intros ?????. iIntros "Hwp".
-  wp_rec. wp_pures. iFrame.
+  wp_call. iFrame.
 Qed.
 
 Global Instance pure_exception_do_return_v (v : val) : PureWp True (exception_do (return_val v)%E) (v).
 Proof.
   rewrite exception_do_unseal return_val_unseal.
   intros ?????. iIntros "Hwp".
-  wp_rec. wp_pures. iFrame.
+  wp_call. iFrame.
 Qed.
 
 Global Instance pure_exception_do_execute_v (v : val) :
@@ -46,6 +49,6 @@ Global Instance pure_exception_do_execute_v (v : val) :
 Proof.
   rewrite exception_do_unseal execute_val_unseal.
   intros ?????. iIntros "Hwp".
-  wp_rec. wp_pures. iFrame.
+  wp_call. iFrame.
 Qed.
 End wps.
